Rewriting E' in terms of the rest of the variables.
$$\begin{align}
\dfrac{1}{E'}-\dfrac{1}{E} &= \dfrac{1}{m_ec^2}\left(1-\cos\theta\right)\\
\implies \dfrac{1}{E'} &= \dfrac{1}{m_ec^2}\left(1-\cos\theta\right)+\dfrac{1}{E}\\
\implies \dfrac{1}{E'} &= \dfrac{E}{Em_ec^2}\left(1-\cos\theta\right)+\dfrac{m_ec^2}{Em_ec^2}\\
\implies \dfrac{1}{E'} &= \dfrac{E\left(1-\cos\theta\right)+m_ec^2}{Em_ec^2}\\
\implies \Aboxed{E' &= E\cdot\dfrac{m_ec^2}{E\left(1-\cos\theta\right)+m_ec^2}}\\
\end{align}$$
The kinetic energy of the electron can then be expressed as:
$$\begin{align}
E-E' &= E-E\cdot\dfrac{m_ec^2}{E\left(1-\cos\theta\right)+m_ec^2}\\
&= E\left(1-\dfrac{m_ec^2}{E\left(1-\cos\theta\right)+m_ec^2}\right)\\
&= E\left(\dfrac{E\left(1-\cos\theta\right)+m_ec^2-m_ec^2}{E\left(1-\cos\theta\right)+m_ec^2}\right)\\
\mathrm{KE}_{e}&= E\left(\dfrac{E\left(1-\cos\theta\right)}{E\left(1-\cos\theta\right)+m_ec^2}\right)\\
\Aboxed{\mathrm{KE}_{e}&= E\left(1+\dfrac{m_ec^2}{E\left(1-\cos\theta\right)}\right)^{-1}}
\end{align}$$


